Simplify SimSTS

simulations/simglobal/SimSTS.v
@@ -6,115 +6,114 @@ Set Implicit Arguments.
 
 Section BEHAVES.
 
-Variable L: semantics.
+  Variable L: semantics.
 
-Theorem of_state_ind2 :
-forall (P: _ -> _ -> Prop),
-(forall st0 retv, state_sort L st0 = final retv -> P st0 (Tr.done retv)) ->
-(forall st0, Beh.state_spin L st0 -> P st0 Tr.spin) ->
-(forall st0, P st0 Tr.nb) ->
+  Theorem of_state_ind2 :
+    forall (P: _ -> _ -> Prop),
+      (forall st0 retv, state_sort L st0 = final retv -> P st0 (Tr.done retv)) ->
+      (forall st0, Beh.state_spin L st0 -> P st0 Tr.spin) ->
+      (forall st0, P st0 Tr.nb) ->
 
-(forall st0 st1 ev evs
- (SRT: state_sort L st0 = vis)
- (STEP: _.(step) st0 (Some ev) st1)
- (TL: Beh.of_state L st1 evs)
-  ,
-    P st0 (Tr.cons ev evs)) ->
-(forall st0 evs
- (SRT: state_sort L st0 = demonic)
- (STEP: Beh.union L st0
-   (fun e st1 =>
-    <<HD: e = None >> /\ <<TL: Beh.of_state L st1 evs >> /\ <<IH: P st1 evs>>)), P st0 evs) ->
-(forall st0 evs
-        (* (IH: forall st1 (STEP: L.(step) st0 None st1), P st1 evs) *)
- (SRT: state_sort L st0 = angelic)
- (STEP: Beh.inter L st0
-   (fun e st1 => <<HD: e = None >> /\ <<TL: Beh.of_state L st1 evs >> /\ <<IH: P st1 evs>>)),
- P st0 evs) ->
-forall s t, Beh.of_state L s t -> P s t.
-Proof.
-  i. eapply Beh.of_state_ind; eauto.
-  { i. eapply H3; eauto.
-    unfold Beh.union in *. des. esplits; eauto.
-    pfold. eapply Beh.of_state_mon; eauto.
-  }
-  { i. eapply H4; eauto. ii. exploit STEP; eauto.
-    i. des. esplits; eauto.
-    pfold. eapply Beh.of_state_mon; eauto.
-  }
-  { punfold H5. eapply Beh.of_state_mon; eauto.
-    i. pclearbot. auto.
-  }
-Qed.
+      (forall st0 st1 ev evs
+              (SRT: state_sort L st0 = vis)
+              (STEP: _.(step) st0 (Some ev) st1)
+              (TL: Beh.of_state L st1 evs)
+        ,
+          P st0 (Tr.cons ev evs)) ->
+      (forall st0 evs
+              (SRT: state_sort L st0 = demonic)
+              (STEP: Beh.union L st0
+                       (fun e st1 =>
+                          <<HD: e = None >> /\ <<TL: Beh.of_state L st1 evs >> /\ <<IH: P st1 evs>>)), P st0 evs) ->
+      (forall st0 evs
+              (SRT: state_sort L st0 = angelic)
+              (STEP: Beh.inter L st0
+                       (fun e st1 => <<HD: e = None >> /\ <<TL: Beh.of_state L st1 evs >> /\ <<IH: P st1 evs>>)),
+          P st0 evs) ->
+      forall s t, Beh.of_state L s t -> P s t.
+  Proof.
+    i. eapply Beh.of_state_ind; eauto.
+    { i. eapply H3; eauto.
+      unfold Beh.union in *. des. esplits; eauto.
+      pfold. eapply Beh.of_state_mon; eauto.
+    }
+    { i. eapply H4; eauto. ii. exploit STEP; eauto.
+      i. des. esplits; eauto.
+      pfold. eapply Beh.of_state_mon; eauto.
+    }
+    { punfold H5. eapply Beh.of_state_mon; eauto.
+      i. pclearbot. auto.
+    }
+  Qed.
 
-Variant of_state_indC (of_state: L.(state) -> Tr.t -> Prop): L.(state) -> Tr.t -> Prop :=
-| of_state_indC_final
-    st0 retv
-    (FINAL: L.(state_sort) st0 = final retv)
-  :
-    of_state_indC of_state st0 (Tr.done retv)
-| of_state_indC_spin
-    st0
-    (SPIN: Beh.state_spin L st0)
-  :
-    of_state_indC of_state st0 (Tr.spin)
-| of_state_indC_nb
-    st0
-  :
-    of_state_indC of_state st0 (Tr.nb)
-| of_state_indC_vis
-    st0 st1 ev evs
-    (SRT: L.(state_sort) st0 = vis)
-    (STEP: _.(step) st0 (Some ev) st1)
-    (TL: of_state st1 evs)
-  :
-    of_state_indC of_state st0 (Tr.cons ev evs)
-| of_state_indC_demonic
-    st0
-    evs
-    (SRT: L.(state_sort) st0 = demonic)
-    (STEP: Beh.union L st0 (fun e st1 => (<<HD: e = None>>) /\ (<<TL: of_state st1 evs>>)))
-  :
-    of_state_indC of_state st0 evs
-| of_state_indC_angelic
-    st0
-    evs
-    (SRT: L.(state_sort) st0 = angelic)
-    (STEP: Beh.inter L st0 (fun e st1 => (<<HD: e = None>>) /\ (<<TL: of_state st1 evs>>)))
-  :
-    of_state_indC of_state st0 evs
-.
+  Variant of_state_indC (of_state: L.(state) -> Tr.t -> Prop): L.(state) -> Tr.t -> Prop :=
+    | of_state_indC_final
+        st0 retv
+        (FINAL: L.(state_sort) st0 = final retv)
+      :
+      of_state_indC of_state st0 (Tr.done retv)
+    | of_state_indC_spin
+        st0
+        (SPIN: Beh.state_spin L st0)
+      :
+      of_state_indC of_state st0 (Tr.spin)
+    | of_state_indC_nb
+        st0
+      :
+      of_state_indC of_state st0 (Tr.nb)
+    | of_state_indC_vis
+        st0 st1 ev evs
+        (SRT: L.(state_sort) st0 = vis)
+        (STEP: _.(step) st0 (Some ev) st1)
+        (TL: of_state st1 evs)
+      :
+      of_state_indC of_state st0 (Tr.cons ev evs)
+    | of_state_indC_demonic
+        st0
+        evs
+        (SRT: L.(state_sort) st0 = demonic)
+        (STEP: Beh.union L st0 (fun e st1 => (<<HD: e = None>>) /\ (<<TL: of_state st1 evs>>)))
+      :
+      of_state_indC of_state st0 evs
+    | of_state_indC_angelic
+        st0
+        evs
+        (SRT: L.(state_sort) st0 = angelic)
+        (STEP: Beh.inter L st0 (fun e st1 => (<<HD: e = None>>) /\ (<<TL: of_state st1 evs>>)))
+      :
+      of_state_indC of_state st0 evs
+  .
 
-Lemma of_state_indC_mon:
-  monotone2 of_state_indC.
-Proof.
-  ii. inv IN; eauto.
-  - econs 1; eauto.
-  - econs 2; eauto.
-  - econs 3; eauto.
-  - econs 4; eauto.
-  - econs 5; eauto. unfold Beh.union in *. des. esplits; eauto.
-  - econs 6; eauto. ii. exploit STEP; eauto. i. des. splits; auto.
-Qed.
-Hint Resolve of_state_indC_mon: paco.
+  Lemma of_state_indC_mon:
+    monotone2 of_state_indC.
+  Proof.
+    ii. inv IN; eauto.
+    - econs 1; eauto.
+    - econs 2; eauto.
+    - econs 3; eauto.
+    - econs 4; eauto.
+    - econs 5; eauto. unfold Beh.union in *. des. esplits; eauto.
+    - econs 6; eauto. ii. exploit STEP; eauto. i. des. splits; auto.
+  Qed.
+  Hint Resolve of_state_indC_mon: paco.
 
-Lemma of_state_indC_spec:
-  of_state_indC <3= gupaco2 (Beh._of_state L) (cpn2 (Beh._of_state L)).
-Proof.
-  eapply wrespect2_uclo; eauto with paco.
-  econs; eauto with paco.
-  ii. inv PR.
-  { econs 1; eauto. }
-  { econs 2; eauto. }
-  { econs 3; eauto. }
-  { econs 4; eauto. eapply rclo2_base. auto. }
-  { econs 5; eauto. unfold Beh.union in *. des. esplits; eauto.
-    eapply Beh.of_state_mon; eauto. i. eapply rclo2_base. auto.
-  }
-  { econs 6; eauto. ii. exploit STEP; eauto. i. des. splits; auto.
-    eapply Beh.of_state_mon; eauto. i. eapply rclo2_base. auto.
-  }
-Qed.
+  Lemma of_state_indC_spec:
+    of_state_indC <3= gupaco2 (Beh._of_state L) (cpn2 (Beh._of_state L)).
+  Proof.
+    eapply wrespect2_uclo; eauto with paco.
+    econs; eauto with paco.
+    ii. inv PR.
+    { econs 1; eauto. }
+    { econs 2; eauto. }
+    { econs 3; eauto. }
+    { econs 4; eauto. eapply rclo2_base. auto. }
+    { econs 5; eauto. unfold Beh.union in *. des. esplits; eauto.
+      eapply Beh.of_state_mon; eauto. i. eapply rclo2_base. auto.
+    }
+    { econs 6; eauto. ii. exploit STEP; eauto. i. des. splits; auto.
+      eapply Beh.of_state_mon; eauto. i. eapply rclo2_base. auto.
+    }
+  Qed.
 
 End BEHAVES.
 
@@ -152,163 +151,89 @@ Proof.
   exploit STEP0; et. i; des. pclearbot. et.
 Qed.
 
-
-
 Section SIM.
 
   Variable L0 L1: semantics.
 
-  Inductive _sim (sim: bool -> bool -> L0.(state) -> L1.(state) -> Prop)
-            (i_src0: bool) (i_tgt0: bool) (st_src0: L0.(state)) (st_tgt0: L1.(state)): Prop :=
+  Variant sim_def (sim: bool -> bool -> L0.(state) -> L1.(state) -> Prop)
+    (self: bool -> bool -> L0.(state) -> L1.(state) -> Prop)
+    (ps0: bool) (pt0: bool) (st_src0: L0.(state)) (st_tgt0: L1.(state)): Prop :=
   | sim_fin
       retv
       (SRT: _.(state_sort) st_src0 = final retv)
       (SRT: _.(state_sort) st_tgt0 = final retv)
-    :
-      _sim sim i_src0 i_tgt0 st_src0 st_tgt0
 
   | sim_vis
       (SRT: _.(state_sort) st_src0 = vis)
       (SRT: _.(state_sort) st_tgt0 = vis)
       (SIM: forall ev st_tgt1
           (STEP: _.(step) st_tgt0 (Some ev) st_tgt1)
-        ,
+          ,
           exists st_src1 (STEP: _.(step) st_src0 (Some ev) st_src1),
             <<SIM: sim true true st_src1 st_tgt1>>)
-    :
-      _sim sim i_src0 i_tgt0 st_src0 st_tgt0
 
   | sim_vis_stuck_tgt
       (SRT: _.(state_sort) st_tgt0 = vis)
       (STUCK: forall ev st_tgt1, not (_.(step) st_tgt0 (Some ev) st_tgt1))
-    :
-      _sim sim i_src0 i_tgt0 st_src0 st_tgt0
 
   | sim_demonic_src
       (SRT: _.(state_sort) st_src0 = demonic)
       (SIM: exists st_src1
                    (STEP: _.(step) st_src0 None st_src1)
         ,
-          <<SIM: _sim sim true i_tgt0 st_src1 st_tgt0>>)
-    :
-      _sim sim i_src0 i_tgt0 st_src0 st_tgt0
+          <<SIM: self true pt0 st_src1 st_tgt0>>)
+
   | sim_demonic_tgt
       (SRT: _.(state_sort) st_tgt0 = demonic)
       (SIM: forall st_tgt1
                    (STEP: _.(step) st_tgt0 None st_tgt1)
         ,
-          <<SIM: _sim sim i_src0 true st_src0 st_tgt1>>)
-    :
-      _sim sim i_src0 i_tgt0 st_src0 st_tgt0
+          <<SIM: self ps0 true st_src0 st_tgt1>>)
+
   | sim_angelic_src
       (SRT: _.(state_sort) st_src0 = angelic)
       (SIM: forall st_src1
           (STEP: _.(step) st_src0 None st_src1)
         ,
-          <<SIM: _sim sim true i_tgt0 st_src1 st_tgt0>>)
-    :
-      _sim sim i_src0 i_tgt0 st_src0 st_tgt0
+          <<SIM: self true pt0 st_src1 st_tgt0>>)
+
   | sim_angelic_tgt
       (SRT: _.(state_sort) st_tgt0 = angelic)
       (SIM: exists st_tgt1
           (STEP: _.(step) st_tgt0 None st_tgt1)
         ,
-          <<SIM: _sim sim i_src0 true st_src0 st_tgt1>>)
-    :
-      _sim sim i_src0 i_tgt0 st_src0 st_tgt0
+          <<SIM: self ps0 true st_src0 st_tgt1>>)
 
   | sim_progress
       (SIM: sim false false st_src0 st_tgt0)
-      (SRC: i_src0 = true)
-      (TGT: i_tgt0 = true)
-    :
-      _sim sim i_src0 i_tgt0 st_src0 st_tgt0
+      (SRC: ps0 = true)
+      (TGT: pt0 = true)
   .
 
-  Lemma _sim_ind2 sim (P: bool -> bool -> L0.(state) -> L1.(state) -> Prop)
-        (FIN: forall
-            i_src0 i_tgt0 st_src0 st_tgt0
-            retv
-            (SRT: _.(state_sort) st_src0 = final retv)
-            (SRT: _.(state_sort) st_tgt0 = final retv),
-            P i_src0 i_tgt0 st_src0 st_tgt0)
-        (VIS: forall
-            i_src0 i_tgt0 st_src0 st_tgt0
-            (SRT: _.(state_sort) st_src0 = vis)
-            (SRT: _.(state_sort) st_tgt0 = vis)
-            (SIM: forall ev st_tgt1
-                         (STEP: _.(step) st_tgt0 (Some ev) st_tgt1)
-              ,
-                exists st_src1 (STEP: _.(step) st_src0 (Some ev) st_src1),
-                  <<SIM: sim true true st_src1 st_tgt1>>),
-            P i_src0 i_tgt0 st_src0 st_tgt0)
-        (VISSTUCK: forall
-            i_src0 i_tgt0 st_src0 st_tgt0
-            (SRT: _.(state_sort) st_tgt0 = vis)
-            (STUCK: forall ev st_tgt1, not (_.(step) st_tgt0 (Some ev) st_tgt1)),
-            P i_src0 i_tgt0 st_src0 st_tgt0)
-        (DMSRC: forall
-            i_src0 i_tgt0 st_src0 st_tgt0
-            (SRT: _.(state_sort) st_src0 = demonic)
-            (SIM: exists st_src1
-                         (STEP: _.(step) st_src0 None st_src1)
-              ,
-                <<SIM: _sim sim true i_tgt0 st_src1 st_tgt0>> /\ <<IH: P true i_tgt0 st_src1 st_tgt0>>),
-            P i_src0 i_tgt0 st_src0 st_tgt0)
-        (DMTGT: forall
-            i_src0 i_tgt0 st_src0 st_tgt0
-            (SRT: _.(state_sort) st_tgt0 = demonic)
-            (SIM: forall st_tgt1
-                         (STEP: _.(step) st_tgt0 None st_tgt1)
-              ,
-                <<SIM: _sim sim i_src0 true st_src0 st_tgt1>> /\ <<IH: P i_src0 true st_src0 st_tgt1>>),
-            P i_src0 i_tgt0 st_src0 st_tgt0)
-        (ANSRC: forall
-            i_src0 i_tgt0 st_src0 st_tgt0
-            (SRT: _.(state_sort) st_src0 = angelic)
-            (SIM: forall st_src1
-                         (STEP: _.(step) st_src0 None st_src1)
-              ,
-                <<SIM: _sim sim true i_tgt0 st_src1 st_tgt0>> /\ <<IH: P true i_tgt0 st_src1 st_tgt0>>),
-            P i_src0 i_tgt0 st_src0 st_tgt0)
-        (ANTGT: forall
-            i_src0 i_tgt0 st_src0 st_tgt0
-            (SRT: _.(state_sort) st_tgt0 = angelic)
-            (SIM: exists st_tgt1
-                         (STEP: _.(step) st_tgt0 None st_tgt1)
-              ,
-                <<SIM: _sim sim i_src0 true st_src0 st_tgt1>> /\ <<IH: P i_src0 true st_src0 st_tgt1>>),
-            P i_src0 i_tgt0 st_src0 st_tgt0)
-        (PROGRESS:
-           forall
-             i_src0 i_tgt0 st_src0 st_tgt0
-             (SIM: sim false false st_src0 st_tgt0)
-             (SRC: i_src0 = true)
-             (TGT: i_tgt0 = true),
-             P i_src0 i_tgt0 st_src0 st_tgt0)
+  Inductive _sim sim ps pt st_src st_tgt : Prop :=
+    _sim_intro (SIM: sim_def sim (_sim sim) ps pt st_src st_tgt)
+  .
+
+  Lemma sim_ind sim (P: bool -> bool -> L0.(state) -> L1.(state) -> Prop)
+    (SIM: sim_def sim (_sim sim /4\ P) <4= P)
     :
-      forall i_src0 i_tgt0 st_src0 st_tgt0
-             (SIM: _sim sim i_src0 i_tgt0 st_src0 st_tgt0),
-        P i_src0 i_tgt0 st_src0 st_tgt0.
+    _sim sim <4= P.
   Proof.
-    fix IH 5. i. inv SIM.
-    { eapply FIN; eauto. }
-    { eapply VIS; eauto. }
-    { eapply VISSTUCK; eauto. }
-    { eapply DMSRC; eauto.
-      des. esplits; eauto. }
-    { eapply DMTGT; eauto. i.
-      hexploit SIM0; eauto. }
-    { eapply ANSRC; eauto. i.
-      hexploit SIM0; eauto. }
-    { eapply ANTGT; eauto.
-      des. esplits; eauto. }
-    { eapply PROGRESS; eauto. }
+    fix IH 5. i. inv PR. inv SIM0; des.
+    - eapply SIM. econs 1; eauto 7.
+    - eapply SIM. econs 2; eauto 7.
+    - eapply SIM. econs 3; eauto 7.
+    - eapply SIM. econs 4; eauto 7.
+    - eapply SIM. econs 5; eauto. i. hexploit SIM1; eauto.
+    - eapply SIM. econs 6; eauto. i. hexploit SIM1; eauto.
+    - eapply SIM. econs 7; eauto 7.
+    - eapply SIM. econs 8; eauto 7.
   Qed.
 
   Lemma sim_mon: monotone4 _sim.
   Proof.
-    ii. revert x0 x1 x2 x3 IN. eapply _sim_ind2; i; clarify.
+    ii. revert x0 x1 x2 x3 IN. eapply sim_ind. i.
+    inv PR; clarify; econs.
     { econs 1; eauto. }
     { econs 2; eauto. i. exploit SIM; eauto. i. des. esplits; eauto. }
     { econs 3; eauto. }
@@ -326,153 +251,8 @@ Section SIM.
   Hint Resolve sim_mon: paco.
   Hint Resolve cpn4_wcompat: paco.
 
-  Lemma sim_ind (P: bool -> bool -> L0.(state) -> L1.(state) -> Prop)
-        (FIN: forall
-            i_src0 i_tgt0 st_src0 st_tgt0
-            retv
-            (SRT: _.(state_sort) st_src0 = final retv)
-            (SRT: _.(state_sort) st_tgt0 = final retv),
-            P i_src0 i_tgt0 st_src0 st_tgt0)
-        (VIS: forall
-            i_src0 i_tgt0 st_src0 st_tgt0
-            (SRT: _.(state_sort) st_src0 = vis)
-            (SRT: _.(state_sort) st_tgt0 = vis)
-            (SIM: forall ev st_tgt1
-                         (STEP: _.(step) st_tgt0 (Some ev) st_tgt1)
-              ,
-                exists st_src1 (STEP: _.(step) st_src0 (Some ev) st_src1),
-                  <<SIM: sim true true st_src1 st_tgt1>>),
-            P i_src0 i_tgt0 st_src0 st_tgt0)
-        (VISSTUCK: forall
-            i_src0 i_tgt0 st_src0 st_tgt0
-            (SRT: _.(state_sort) st_tgt0 = vis)
-            (STUCK: forall ev st_tgt1, not (_.(step) st_tgt0 (Some ev) st_tgt1)),
-            P i_src0 i_tgt0 st_src0 st_tgt0)
-        (DMSRC: forall
-            i_src0 i_tgt0 st_src0 st_tgt0
-            (SRT: _.(state_sort) st_src0 = demonic)
-            (SIM: exists st_src1
-                         (STEP: _.(step) st_src0 None st_src1)
-              ,
-                <<SIM: sim true i_tgt0 st_src1 st_tgt0>> /\ <<IH: P true i_tgt0 st_src1 st_tgt0>>),
-            P i_src0 i_tgt0 st_src0 st_tgt0)
-        (DMTGT: forall
-            i_src0 i_tgt0 st_src0 st_tgt0
-            (SRT: _.(state_sort) st_tgt0 = demonic)
-            (SIM: forall st_tgt1
-                         (STEP: _.(step) st_tgt0 None st_tgt1)
-              ,
-                <<SIM: sim i_src0 true st_src0 st_tgt1>> /\ <<IH: P i_src0 true st_src0 st_tgt1>>),
-            P i_src0 i_tgt0 st_src0 st_tgt0)
-        (ANSRC: forall
-            i_src0 i_tgt0 st_src0 st_tgt0
-            (SRT: _.(state_sort) st_src0 = angelic)
-            (SIM: forall st_src1
-                         (STEP: _.(step) st_src0 None st_src1)
-              ,
-                <<SIM: sim true i_tgt0 st_src1 st_tgt0>> /\ <<IH: P true i_tgt0 st_src1 st_tgt0>>),
-            P i_src0 i_tgt0 st_src0 st_tgt0)
-        (ANTGT: forall
-            i_src0 i_tgt0 st_src0 st_tgt0
-            (SRT: _.(state_sort) st_tgt0 = angelic)
-            (SIM: exists st_tgt1
-                         (STEP: _.(step) st_tgt0 None st_tgt1)
-              ,
-                <<SIM: sim i_src0 true st_src0 st_tgt1>> /\ <<IH: P i_src0 true st_src0 st_tgt1>>),
-            P i_src0 i_tgt0 st_src0 st_tgt0)
-        (PROGRESS:
-           forall
-             i_src0 i_tgt0 st_src0 st_tgt0
-             (SIM: sim false false st_src0 st_tgt0)
-             (SRC: i_src0 = true)
-             (TGT: i_tgt0 = true),
-             P i_src0 i_tgt0 st_src0 st_tgt0)
-    :
-      forall i_src0 i_tgt0 st_src0 st_tgt0
-             (SIM: sim i_src0 i_tgt0 st_src0 st_tgt0),
-        P i_src0 i_tgt0 st_src0 st_tgt0.
-  Proof.
-    i. eapply (@_sim_ind2 sim P); eauto.
-    { i. eapply DMSRC; eauto. des. esplits; eauto.
-      pfold. eapply sim_mon; eauto.
-    }
-    { i. eapply DMTGT; eauto. i. hexploit SIM0; eauto. i. des. esplits; eauto.
-      pfold. eapply sim_mon; eauto.
-    }
-    { i. eapply ANSRC; eauto. i. hexploit SIM0; eauto. i. des. esplits; eauto.
-      pfold. eapply sim_mon; eauto.
-    }
-    { i. eapply ANTGT; eauto. des. esplits; eauto.
-      pfold. eapply sim_mon; eauto.
-    }
-    { punfold SIM. eapply sim_mon; eauto. i. pclearbot. auto. }
-  Qed.
-
-  Variant sim_indC (sim: bool -> bool -> L0.(state) -> L1.(state) -> Prop)
-          (i_src0: bool) (i_tgt0: bool) (st_src0: L0.(state)) (st_tgt0: L1.(state)): Prop :=
-  | sim_indC_fin
-      retv
-      (SRT: _.(state_sort) st_src0 = final retv)
-      (SRT: _.(state_sort) st_tgt0 = final retv)
-    :
-      sim_indC sim i_src0 i_tgt0 st_src0 st_tgt0
-
-  | sim_indC_vis
-      (SRT: _.(state_sort) st_src0 = vis)
-      (SRT: _.(state_sort) st_tgt0 = vis)
-      (SIM: forall ev st_tgt1
-          (STEP: _.(step) st_tgt0 (Some ev) st_tgt1)
-        ,
-          exists st_src1 (STEP: _.(step) st_src0 (Some ev) st_src1),
-            <<SIM: sim true true st_src1 st_tgt1>>)
-    :
-      sim_indC sim i_src0 i_tgt0 st_src0 st_tgt0
-
-  | sim_indC_vis_stuck_tgt
-      (SRT: _.(state_sort) st_tgt0 = vis)
-      (STUCK: forall ev st_tgt1, not (_.(step) st_tgt0 (Some ev) st_tgt1))
-    :
-      sim_indC sim i_src0 i_tgt0 st_src0 st_tgt0
-  | sim_indC_demonic_src
-      (SRT: _.(state_sort) st_src0 = demonic)
-      (SIM: exists st_src1
-                   (STEP: _.(step) st_src0 None st_src1)
-        ,
-          <<SIM: sim true i_tgt0 st_src1 st_tgt0>>)
-    :
-      sim_indC sim i_src0 i_tgt0 st_src0 st_tgt0
-  | sim_indC_demonic_tgt
-      (SRT: _.(state_sort) st_tgt0 = demonic)
-      (SIM: forall st_tgt1
-                   (STEP: _.(step) st_tgt0 None st_tgt1)
-        ,
-          <<SIM: sim i_src0 true st_src0 st_tgt1>>)
-    :
-      sim_indC sim i_src0 i_tgt0 st_src0 st_tgt0
-  | sim_indC_angelic_src
-      (SRT: _.(state_sort) st_src0 = angelic)
-      (SIM: forall st_src1
-          (STEP: _.(step) st_src0 None st_src1)
-        ,
-          <<SIM: sim true i_tgt0 st_src1 st_tgt0>>)
-    :
-      sim_indC sim i_src0 i_tgt0 st_src0 st_tgt0
-  | sim_indC_angelic_tgt
-      (SRT: _.(state_sort) st_tgt0 = angelic)
-      (SIM: exists st_tgt1
-          (STEP: _.(step) st_tgt0 None st_tgt1)
-        ,
-          <<SIM: sim i_src0 true st_src0 st_tgt1>>)
-    :
-      sim_indC sim i_src0 i_tgt0 st_src0 st_tgt0
-  | sim_indC_progress
-      (SIM: sim false false st_src0 st_tgt0)
-      (SRC: i_src0 = true)
-      (TGT: i_tgt0 = true)
-    :
-      sim_indC sim i_src0 i_tgt0 st_src0 st_tgt0
-  .
-
+  Definition sim_indC sim := sim_def sim sim.
+  
   Lemma sim_indC_mon: monotone4 sim_indC.
   Proof.
     ii. inv IN; eauto.
@@ -491,7 +271,7 @@ Section SIM.
     sim_indC <5= gupaco4 _sim (cpn4 _sim).
   Proof.
     eapply wrespect4_uclo; eauto with paco.
-    econs; eauto with paco. i. inv PR.
+    econs; eauto with paco. i. inv PR; econs.
     { econs 1; eauto. }
     { econs 2; eauto. i. exploit SIM; eauto. i. des.
       esplits; eauto. eapply rclo4_base. auto. }
@@ -512,12 +292,12 @@ Section SIM.
   Qed.
 
   Variant sim_flagC (sim: bool -> bool -> L0.(state) -> L1.(state) -> Prop)
-          (i_src1: bool) (i_tgt1: bool) (st_src: L0.(state)) (st_tgt: L1.(state)): Prop :=
+          (ps1: bool) (pt1: bool) (st_src: L0.(state)) (st_tgt: L1.(state)): Prop :=
   | sim_flagC_intro
-      i_src0 i_tgt0
-      (SIM: sim i_src0 i_tgt0 st_src st_tgt)
-      (SRC: i_src0 = true -> i_src1 = true)
-      (TGT: i_tgt0 = true -> i_tgt1 = true)
+      ps0 pt0
+      (SIM: sim ps0 pt0 st_src st_tgt)
+      (SRC: ps0 = true -> ps1 = true)
+      (TGT: pt0 = true -> pt1 = true)
   .
 
   Lemma sim_flagC_mon: monotone4 sim_flagC.
@@ -532,14 +312,15 @@ Section SIM.
     eapply wrespect4_uclo; eauto with paco.
     econs; eauto with paco. i. inv PR.
     eapply GF in SIM.
-    revert x0 x1 SRC TGT. induction SIM using _sim_ind2; i; clarify.
+    revert x0 x1 SRC TGT. pattern ps0, pt0, x2, x3.
+    eapply sim_ind, SIM. i; inv PR; clarify; econs.
     { econs 1; eauto. }
-    { econs 2; eauto. i. exploit SIM; eauto. i. des.
+    { econs 2; eauto. i. exploit SIM0; eauto. i. des.
       esplits; eauto. eapply rclo4_base. auto. }
     { econs 3; eauto. }
     { econs 4; eauto. des. esplits; eauto. }
-    { econs 5; eauto. i. exploit SIM; eauto. i. des. eauto. }
-    { econs 6; eauto. i. exploit SIM; eauto. i. des. eauto. }
+    { econs 5; eauto. i. exploit SIM0; eauto. i. des. eauto. }
+    { econs 6; eauto. i. exploit SIM0; eauto. i. des. eauto. }
     { econs 7; eauto. des. esplits; eauto. }
     { econs 8; eauto. eapply rclo4_base. auto. }
   Qed.
@@ -562,8 +343,8 @@ Section SIM.
 
   Ltac pc H := rr in H; desH H; ss.
   Lemma adequacy_spin
-        i_src0 i_tgt0 st_src0 st_tgt0
-        (SIM: sim i_src0 i_tgt0 st_src0 st_tgt0)
+        ps0 pt0 st_src0 st_tgt0
+        (SIM: sim ps0 pt0 st_src0 st_tgt0)
         (SPIN: Beh.state_spin L1 st_tgt0)
     :
       <<SPIN: Beh.state_spin L0 st_src0>>
@@ -571,8 +352,9 @@ Section SIM.
   Proof.
     ginit.
     { i. eapply cpn1_wcompat; eauto. eapply Beh.state_spin_mon. }
-    revert i_src0 i_tgt0 st_src0 st_tgt0 SIM SPIN. gcofix CIH.
-    intros ? ? ? ? SIM. induction SIM using sim_ind; i; clarify.
+    revert ps0 pt0 st_src0 st_tgt0 SIM SPIN. gcofix CIH.
+    intros ? ? ? ? SIM. punfold SIM. pattern ps0, pt0, st_src0, st_tgt0.
+    eapply sim_ind, SIM. i. inv PR; clarify.
     - (** final **)
       exfalso. punfold SPIN. inv SPIN; rewrite SRT0 in *; ss.
     - (** vis **)
@@ -585,21 +367,20 @@ Section SIM.
     - (** dtgt **)
       punfold SPIN. inv SPIN; rewrite SRT in *; ss. des. pclearbot.
       exploit wf_demonic; et; i; clarify.
-      exploit SIM; et. i; des. eapply IH; eauto.
+      exploit SIM0; et. i; des. eauto.
     - (** asrc **)
       gstep. econs 1; eauto. i.
       exploit wf_angelic; et; i; clarify.
-      exploit SIM; eauto.  i. des.
+      exploit SIM0; eauto.  i. des.
       eapply gpaco1_mon; eauto. ss.
     - (** atgt **)
       punfold SPIN. inv SPIN; rewrite SRT in *; ss. des.
-      exploit STEP; eauto. i. pclearbot.
-      eapply IH; eauto.
+      exploit STEP; eauto. i. pclearbot. eauto.
     - (** progress **)
-      remember false in SIM at 1.
-      remember false in SIM at 1.
-      revert Heqb. clear Heqb0. revert SPIN.
-      induction SIM using sim_ind; i; clarify.
+      clear SIM. rename SIM0 into SIM. pclearbot. punfold SIM.
+      remember false in SIM at 1. remember false in SIM at 1.
+      clear Heqb0. revert Heqb SPIN.
+      pattern b, b0, x2, x3. eapply sim_ind, SIM. i. inv PR; clarify.
       + exfalso. punfold SPIN. inv SPIN; rewrite SRT1 in *; clarify.
       + exfalso. punfold SPIN. inv SPIN; rewrite SRT1 in *; clarify.
       + exfalso. punfold SPIN. inv SPIN; rewrite SRT0 in *; ss.
@@ -607,61 +388,66 @@ Section SIM.
         gbase. eapply CIH; eauto.
       + punfold SPIN. inv SPIN; rewrite SRT in *; clarify. des.
         exploit wf_demonic; et; i; clarify. pclearbot.
-        exploit SIM; et. i; des. eapply IH; eauto.
+        exploit SIM0; et. i; des. eauto.
       + gstep. econs 1; auto. i.
         exploit wf_angelic; et; i; clarify.
-        exploit SIM; eauto. i. des.
+        exploit SIM0; eauto. i. des.
         gbase. eapply CIH; eauto.
       + punfold SPIN. inv SPIN; rewrite SRT in *; clarify. des.
         exploit STEP; eauto. i. pclearbot.
-        eapply IH; eauto.
+        eauto.
   Qed.
 
   Lemma adequacy_aux
-        i_src0 i_tgt0 st_src0 st_tgt0
-        (SIM: sim i_src0 i_tgt0 st_src0 st_tgt0)
+        ps0 pt0 st_src0 st_tgt0
+        (SIM: sim ps0 pt0 st_src0 st_tgt0)
     :
       <<IMPR: Beh.improves (Beh.of_state L0 st_src0) (Beh.of_state L1 st_tgt0)>>
   .
   Proof.
     ginit.
     { i. eapply cpn2_wcompat; eauto. eapply Beh.of_state_mon. }
-    revert i_tgt0 i_src0 st_src0 st_tgt0 SIM. gcofix CIH.
+    revert pt0 ps0 st_src0 st_tgt0 SIM. gcofix CIH.
     i. rename x2 into tr.
-    revert i_src0 i_tgt0 st_src0 SIM.
+    revert ps0 pt0 st_src0 SIM.
     induction PR using of_state_ind2; ii; ss; rename st0 into st_tgt0.
     - (** done **)
-      rename H into SRT.
-      revert retv SRT. induction SIM using sim_ind; i; clarify.
-      + rewrite SRT0 in *. clarify. gstep. econs; eauto.
+      rename H into SRT. punfold SIM.
+      revert retv SRT. pattern ps0, pt0, st_src0, st_tgt0.
+      eapply sim_ind, SIM. i. inv PR; clarify.
+      + rewrite SRT in *; clarify. gstep. econs; eauto.
+      + rewrite SRT in *. clarify.
       + rewrite SRT0 in *. clarify.
-      + rewrite SRT0 in *. clarify.
-      + des. exploit IH; eauto. i; des; ss.
+      + des. exploit SIM0; eauto. i; des; ss.
         guclo of_state_indC_spec. econs 5; eauto. red. esplits; eauto.
       + rewrite SRT in *. clarify.
       + guclo of_state_indC_spec. econs 6; eauto. ii.
         exploit wf_angelic; et. i; clarify.
-        exploit SIM; eauto. i. des. splits; auto.
+        exploit SIM0; eauto. i. des. splits; auto.
       + rewrite SRT in *. clarify.
-      + remember false as i_src0 eqn:FLAGSRC in SIM at 1.
-        remember false as i_tgt0 eqn:FLAGTGT in SIM at 1.
+      + clear SIM. rename SIM0 into SIM. pclearbot. punfold SIM.
+        remember false as ps1 eqn:FLAGSRC in SIM at 1.
+        remember false as pt1 eqn:FLAGTGT in SIM at 1.
         clear FLAGSRC. revert FLAGTGT. revert retv SRT.
-        induction SIM using sim_ind; i; try rewrite SRT0 in *; clarify.
+        pattern ps1, pt1, x2, x3.
+        eapply sim_ind, SIM. i. inv PR; try rewrite SRT in *; clarify.
         * gstep. econs; eauto.
         * des. guclo of_state_indC_spec. econs 5; eauto.
           red. esplits; eauto.
         * guclo of_state_indC_spec. econs 6; eauto. ii.
           exploit wf_angelic; et. i; clarify.
-          exploit SIM; eauto. i. des. esplits; eauto.
+          exploit SIM0; eauto. i. des. esplits; eauto.
     - (** spin **)
       exploit adequacy_spin; eauto. i.
       gstep. econs. et.
     - (** nb **)
       gstep. econs; eauto.
     - (** cons **)
-      induction SIM using sim_ind; i; try rewrite SRT in *; clarify.
+      move SIM before CIH. revert_until SIM.
+      punfold SIM. pattern ps0, pt0, st_src0, st_tgt0.
+      eapply sim_ind, SIM. i. inv PR; i; try rewrite SRT in *; clarify.
       + (** vv **)
-        specialize (SIM ev st1). apply SIM in STEP; clear SIM; des.
+        specialize (SIM0 ev st1). apply SIM0 in STEP; clear SIM; des.
         gstep. econs 4; eauto. pc SIM. gbase. eapply CIH; eauto.
       + (** vis stuck **)
         apply STUCK in STEP. clarify.
@@ -670,53 +456,64 @@ Section SIM.
       + (** a_ **)
         guclo of_state_indC_spec. econs 6; eauto. ii.
         exploit wf_angelic; et. i; clarify.
-        exploit SIM; eauto. i. des. esplits; eauto.
+        exploit SIM0; eauto. i. des. esplits; eauto.
       + (** progress **)
-        remember false as i_src0 eqn:FLAGSRC in SIM at 1.
-        remember false as i_tgt0 eqn:FLAGTGT in SIM at 1.
-        clear FLAGSRC. revert FLAGTGT. revert ev SRT STEP.
-        induction SIM using sim_ind; i; try rewrite SRT0 in *; clarify.
-        * exploit SIM; eauto. i. des. gstep. econs 4; eauto. gbase. eauto.
+        clear SIM. rename SIM0 into SIM. pclearbot. punfold SIM.
+        remember false as ps1 eqn:FLAGSRC in SIM at 1.
+        remember false as pt1 eqn:FLAGTGT in SIM at 1.
+        clear FLAGSRC. revert FLAGTGT ev SRT STEP.
+        pattern ps1, pt1, x2, x3. eapply sim_ind, SIM. i.
+        inv PR; try rewrite SRT in *; clarify.
+        * exploit SIM0; eauto. i. des. pclearbot.
+          gstep. econs 4; eauto. gbase. eauto.
         * exfalso. eapply STUCK; eauto.
-        * des. exploit IH; eauto. i.
+        * des. exploit SIM0; eauto. i.
           guclo of_state_indC_spec. econs 5; eauto. red. esplits; eauto.
         * guclo of_state_indC_spec. econs 6; eauto. ii.
           exploit wf_angelic; et. i; clarify.
-          exploit SIM; eauto. i. des. esplits; eauto.
+          exploit SIM0; eauto. i. des. esplits; eauto.
     - (** demonic **)
-      red in STEP. des. clarify.
-      induction SIM using sim_ind; i; try rewrite SRT in *; clarify.
+      red in STEP. des. clarify. punfold SIM.
+      move SIM before CIH. revert_until SIM.
+      pattern ps0, pt0, st_src0, st_tgt0.
+      eapply sim_ind, SIM. i. inv PR; try rewrite SRT in *; clarify.
       + des. guclo of_state_indC_spec. econs 5; eauto. red. esplits; eauto.
-      + hexploit SIM; eauto. i. des. eapply IH; eauto.
+      + hexploit SIM0; eauto. i. des. eapply IH; eauto.
       + guclo of_state_indC_spec. econs 6; eauto. ii.
         exploit wf_angelic; et. i; clarify.
-        exploit SIM; eauto. i. des. esplits; eauto.
-      + remember false as i_src0 eqn:FLAGSRC in SIM at 1.
-        remember false as i_tgt0 eqn:FLAGTGT in SIM at 1.
-        clear FLAGSRC. revert FLAGTGT. revert st1 SRT STEP0 TL IH.
-        induction SIM using sim_ind; i; try rewrite SRT0 in *; clarify.
-        * des. exploit IH0; eauto. i.
+        exploit SIM0; eauto. i. des. esplits; eauto.
+      + clear SIM. rename SIM0 into SIM.
+        remember false as ps1 eqn:FLAGSRC in SIM at 1.
+        remember false as pt1 eqn:FLAGTGT in SIM at 1.
+        clear FLAGSRC. revert FLAGTGT st1 SRT STEP0 TL IH.
+        pclearbot. punfold SIM. pattern ps1, pt1, x2, x3.
+        eapply sim_ind, SIM. i. inv PR; try rewrite SRT in *; clarify.
+        * des. exploit SIM0; eauto. i.
           guclo of_state_indC_spec. econs 5; eauto. red. esplits; eauto.
-        * exploit SIM; eauto. i. des. eapply IH; eauto.
+        * exploit SIM0; eauto. i. des. eapply IH; eauto.
         * guclo of_state_indC_spec. econs 6; eauto. ii.
           exploit wf_angelic; et. i; clarify.
-          exploit SIM; eauto. i. des. esplits; eauto.
+          exploit SIM0; eauto. i. des. esplits; eauto.
     - (** angelic **)
       red in STEP. des. clarify.
-      induction SIM using sim_ind; i; try rewrite SRT in *; clarify.
+      move SIM before CIH. revert_until SIM.
+      punfold SIM. pattern ps0, pt0, st_src0, st_tgt0.
+      eapply sim_ind, SIM. i. inv PR; try rewrite SRT in *; clarify.
       + des. guclo of_state_indC_spec. econs 5; eauto. red. esplits; eauto.
       + guclo of_state_indC_spec. econs 6; eauto. ii.
         exploit wf_angelic; et. i; clarify.
-        exploit SIM; eauto. i. des. esplits; eauto.
+        exploit SIM0; eauto. i. des. esplits; eauto.
       + des. exploit STEP; eauto. i. des. esplits; eauto.
-      + remember false as i_src0 eqn:FLAGSRC in SIM at 1.
-        remember false as i_tgt0 eqn:FLAGTGT in SIM at 1.
-        clear FLAGSRC. revert FLAGTGT. revert SRT STEP.
-        induction SIM using sim_ind; i; try rewrite SRT0 in *; clarify.
+      + clear SIM. rename SIM0 into SIM.
+        remember false as ps1 eqn:FLAGSRC in SIM at 1.
+        remember false as pt1 eqn:FLAGTGT in SIM at 1.
+        clear FLAGSRC. revert FLAGTGT SRT STEP.
+        pclearbot. punfold SIM. pattern ps1, pt1, x2, x3.
+        eapply sim_ind, SIM. i. inv PR; try rewrite SRT in *; clarify.
         * des. guclo of_state_indC_spec. econs 5; eauto. red. esplits; eauto.
         * guclo of_state_indC_spec. econs 6; eauto. ii.
-          exploit wf_angelic; try apply SRT; et. i; clarify.
-          exploit SIM; eauto. i. des. esplits; eauto.
+          exploit wf_angelic; try apply SRT0; et. i; clarify.
+          exploit SIM0; eauto. i. des. esplits; eauto.
         * des. exploit STEP; eauto. i. des. esplits; eauto.
   Qed.
 
