simulations/simglobal/SimGlobalFacts.v
@@ -34,36 +34,36 @@ Section ADEQUACY.
     pattern ps, pt, itr_src, itr_tgt.
     eapply simg_ind, SIM. i.
     depdes PR; i; subst.
-    { gstep. eapply sim_fin; ss; cbn; des_ifs. }
-    { gstep. eapply sim_vis; try by ss. i.
+    { gstep. econs. eapply sim_fin; ss; cbn; des_ifs. }
+    { gstep. econs. eapply sim_vis; try by ss. i.
       eapply step_trigger_io_iff in STEP. des. subst. inv STEP0.
       esplits.
       + eapply step_trigger_io; et.
       + guclo sim_flagC_spec. econs; [gbase; eapply CIH, SIM0|..]; eauto.
     }
-    { guclo sim_indC_spec. eapply sim_indC_demonic_src; try by ss.
+    { guclo sim_indC_spec. eapply sim_demonic_src; try by ss.
       esplits.
       + eapply step_tau; et.
       + guclo sim_flagC_spec. econs; [eapply gpaco4_mon; [eapply SIM0|..]|..]; et; ss.
     }
-    { guclo sim_indC_spec. eapply sim_indC_demonic_tgt; try by ss. i.
+    { guclo sim_indC_spec. eapply sim_demonic_tgt; try by ss. i.
       eapply step_tau_iff in STEP. des. subst.
       guclo sim_flagC_spec. econs; [eapply gpaco4_mon; [eapply SIM1|..]|..]; et; ss.
     }
-    { des. guclo sim_indC_spec. eapply sim_indC_demonic_src; try by ss.
+    { des. guclo sim_indC_spec. eapply sim_demonic_src; try by ss.
       esplits.
       + eapply step_trigger_choose; et.
       + guclo sim_flagC_spec. econs; [eapply gpaco4_mon; [eapply SIM1|..]|..]; et; ss.
     }
-    { guclo sim_indC_spec. eapply sim_indC_demonic_tgt; try by ss.
+    { guclo sim_indC_spec. eapply sim_demonic_tgt; try by ss.
       i. eapply step_trigger_choose_iff in STEP. des. subst.
       guclo sim_flagC_spec. econs; [eapply gpaco4_mon; [eapply SIM0|..]|..]; et; ss.
     }
-    { guclo sim_indC_spec. eapply sim_indC_angelic_src; try by ss.
+    { guclo sim_indC_spec. eapply sim_angelic_src; try by ss.
       i. eapply step_trigger_take_iff in STEP. des. subst.
       guclo sim_flagC_spec. econs; [eapply gpaco4_mon; [eapply SIM0|..]|..]; et; ss.
     }
-    { des. guclo sim_indC_spec. eapply sim_indC_angelic_tgt; try by ss.
+    { des. guclo sim_indC_spec. eapply sim_angelic_tgt; try by ss.
       esplits.
       + eapply step_trigger_take; et.
       + guclo sim_flagC_spec. econs; [eapply gpaco4_mon; [eapply SIM1|..]|..]; et; ss.
@@ -81,43 +81,43 @@ Section ADEQUACY.
     pattern ps, pt, itr_src, itr_tgt.
     eapply simg_ind, SIM. i.
     depdes PR; i; subst.
-    { gstep. eapply sim_fin; ss; cbn; des_ifs. }
-    { gstep. eapply sim_vis; try by ss. i.
+    { gstep. econs. eapply sim_fin; ss; cbn; des_ifs. }
+    { gstep. econs. eapply sim_vis; try by ss. i.
       eapply step_trigger_io_iff in STEP. des. subst. inv STEP0.
       esplits.
       + eapply step_trigger_io; et.
       + guclo sim_flagC_spec. econs; [gbase; eapply CIH, SIM0|..]; eauto.
     }
-    { guclo sim_indC_spec. eapply sim_indC_demonic_src; try by ss.
+    { guclo sim_indC_spec. eapply sim_demonic_src; try by ss.
       esplits.
       + eapply step_tau; et.
       + guclo sim_flagC_spec. econs; [eapply gpaco4_mon; [eapply SIM0|..]|..]; et; ss.
     }
-    { guclo sim_indC_spec. eapply sim_indC_demonic_tgt; try by ss. i.
+    { guclo sim_indC_spec. eapply sim_demonic_tgt; try by ss. i.
       eapply step_tau_iff in STEP. des. subst.
       guclo sim_flagC_spec. econs; [eapply gpaco4_mon; [eapply SIM1|..]|..]; et; ss.
     }
-    { des. guclo sim_indC_spec. eapply sim_indC_demonic_src; try by ss.
+    { des. guclo sim_indC_spec. eapply sim_demonic_src; try by ss.
       esplits.
       + eapply step_trigger_choose; et.
       + guclo sim_flagC_spec. econs; [eapply gpaco4_mon; [eapply SIM1|..]|..]; et; ss.
     }
-    { guclo sim_indC_spec. eapply sim_indC_demonic_tgt; try by ss.
+    { guclo sim_indC_spec. eapply sim_demonic_tgt; try by ss.
       i. eapply step_trigger_choose_iff in STEP. des. subst.
       guclo sim_flagC_spec. econs; [eapply gpaco4_mon; [eapply SIM0|..]|..]; et; ss.
     }
-    { guclo sim_indC_spec. eapply sim_indC_angelic_src; try by ss.
+    { guclo sim_indC_spec. eapply sim_angelic_src; try by ss.
       i. eapply step_trigger_take_iff in STEP. des. subst.
       guclo sim_flagC_spec. econs; [eapply gpaco4_mon; [eapply SIM0|..]|..]; et; ss.
     }
-    { des. guclo sim_indC_spec. eapply sim_indC_angelic_tgt; try by ss.
+    { des. guclo sim_indC_spec. eapply sim_angelic_tgt; try by ss.
       esplits.
       + eapply step_trigger_take; et.
       + guclo sim_flagC_spec. econs; [eapply gpaco4_mon; [eapply SIM1|..]|..]; et; ss.
     }
 
     unfold smj_leb in *.
-    gstep. eapply sim_progress.
+    gstep. econs. eapply sim_progress.
     - gbase. eapply CIH in SIM0.
       destruct ps1, pt1; ss. destruct b, b0; ss.
     - destruct ps0; ss. destruct b; ss. destruct ps1; ss. destruct b; ss.
